cryptis/primitives/sms.v
@@ -1,0 +1,199 @@
+(* HeapLang implementations of the signed-multiset operations from
+   [cryptis.lib.sms], parameterised by HeapLang closures for the element
+   operations: an equality test [eq], the involution [inv], and (for [to]) an
+   order comparison [le].  They mirror the pre-term counterparts in
+   [primitives/pre_term.v] ([hl_insert_exp], [hl_cancel_invs], and the
+   [insertion_sort]-of-[hl_cancel_invs] pattern in [hl_mul]/[hl_exp]) and reuse
+   the shared [insertion_sort] of [lib/list.v] for [to].
+
+   Each implementation gets a continuation-style spec relating it to the pure
+   [SMS.*] model (same shape as the [twp_hl_*] specs in [pre_term.v]). *)
+
+From cryptis Require Import lib.
+From mathcomp Require Import ssreflect.
+From mathcomp Require all_order path.
+From stdpp Require Import sorting list.
+From iris.heap_lang Require Import notation proofmode.
+From cryptis.lib Require Import list_sort sms.
+From cryptis.primitives Require Import notations.
+
+Set Implicit Arguments.
+Unset Strict Implicit.
+Unset Printing Implicit Defensive.
+
+(** ** Implementations *)
+
+Definition sms_insert : val := λ: "eq" "inv" "x" "xs",
+  if: mem_list "eq" ("inv" "x") "xs" then rem_list "eq" ("inv" "x") "xs"
+  else "x" :: "xs".
+
+Definition sms_cancel : val := λ: "eq" "inv" "xs",
+  foldr_list (λ: "x" "acc", sms_insert "eq" "inv" "x" "acc") [] "xs".
+
+Definition sms_to : val := λ: "le" "eq" "inv" "xs",
+  insertion_sort "le" (sms_cancel "eq" "inv" "xs").
+
+Section Proofs.
+
+Context `{!heapGS Σ}.
+Context {T : Type} `{!Repr T, !EqDecision T}.
+Context (i : T -> T) (eqv invv : val).
+
+Hypothesis eqvP : forall (x y : T) E Ψ,
+  Ψ #(bool_decide (x = y)) ⊢ WP eqv (repr x) (repr y) @ E [{ Ψ }].
+Hypothesis invvP : forall (x : T) E Ψ,
+  Ψ (repr (i x)) ⊢ WP invv (repr x) @ E [{ Ψ }].
+
+Implicit Types (x y z : T) (xs ys : list T).
+
+(** ** Membership and removal, stdpp-flavoured *)
+
+Lemma find_mem x xs :
+  bool_decide (x ∈ xs)
+  = match find (fun y => bool_decide (x = y)) xs with Some _ => true | None => false end.
+Proof.
+elim: xs => [|y xs IH].
+- done.
+- rewrite /=; case: (bool_decide_reflect (x = y)) => [->|ne].
+  + by rewrite bool_decide_eq_true_2 //; exact: list_elem_of_here.
+  + rewrite -IH; apply: bool_decide_ext; rewrite elem_of_cons; naive_solver.
+Qed.
+
+Lemma twp_sms_mem x xs E :
+  [[{ True }]] mem_list eqv (repr x) (repr xs) @ E [[{ RET #(bool_decide (x ∈ xs)); True }]].
+Proof.
+iIntros "%Φ _ HΦ"; wp_lam; wp_pures.
+wp_apply twp_find_list => //.
+{ by iIntros "%y %Ψ _ HΨ"; wp_pures; wp_apply eqvP; iApply "HΨ". }
+iIntros "_"; rewrite find_mem.
+by case: (find (fun y => bool_decide (x = y)) xs) => [y|]; wp_pures; iApply "HΦ".
+Qed.
+
+Lemma twp_sms_rem x xs E :
+  [[{ True }]] rem_list eqv (repr x) (repr xs) @ E [[{ RET repr (rem x xs); True }]].
+Proof.
+rewrite repr_list_unseal /=.
+iIntros "%Φ _ HΦ".
+iStopProof; elim: xs Φ => [| y xs IH] Φ /=; iIntros "HΦ"; wp_rec; wp_pures.
+  by iApply "HΦ".
+wp_apply eqvP.
+rewrite (_ : bool_decide (x = y) = bool_decide (y = x)); last first.
+  by apply: bool_decide_ext; split; congruence.
+case: (bool_decide (y = x)) => /=; wp_pures; first by iApply "HΦ".
+wp_apply IH; iIntros "_".
+wp_pures; by iApply "HΦ".
+Qed.
+
+(** ** [insert] and [cancel] *)
+
+Lemma twp_sms_insert x xs E Ψ :
+  Ψ (repr (SMS.insert i x xs)) ⊢ WP sms_insert eqv invv (repr x) (repr xs) @ E [{ Ψ }].
+Proof.
+iIntros "HΨ"; rewrite /SMS.insert; wp_lam; wp_pures.
+wp_apply invvP; wp_apply twp_sms_mem => //; iIntros "_".
+case: (bool_decide (i x ∈ xs)); wp_pures.
+- wp_apply invvP; wp_apply twp_sms_rem => //; iIntros "_"; by iApply "HΨ".
+- wp_apply twp_cons; by iApply "HΨ".
+Qed.
+
+Lemma twp_sms_cancel xs E Ψ :
+  Ψ (repr (SMS.cancel i xs)) ⊢ WP sms_cancel eqv invv (repr xs) @ E [{ Ψ }].
+Proof.
+iIntros "HΨ"; wp_lam; wp_pures.
+wp_apply twp_nil.
+wp_apply twp_foldr_list => //.
+iIntros "%b %a %Φ _ HΦ"; wp_pures; wp_apply twp_sms_insert; by iApply "HΦ".
+iIntros "_"; by iApply "HΨ".
+Qed.
+
+End Proofs.
+
+(** ** [to]: cancel, then sort with the shared [insertion_sort]
+
+    [lib/list.v] proves [insertion_sort] correct only in mathcomp terms
+    ([twp_insertion_sort], phrased with [path.sort] over an [orderType]).  We
+    restate that correctness in stdpp terms — [insertion_sort] computes
+    [merge_sort ole] for the total decidable order [ole] induced by the
+    [orderType] — via the bridge [sort_merge_sort_ole], and use it for [to].
+    Once [twp_insertion_sort] itself is restated over a stdpp order, this
+    [orderType] scaffolding (and the [ole] instances) should be removed. *)
+
+Section Ordered.
+
+#[warnings="-ambiguous-paths"]
+Import all_order path Order.POrderTheory Order.TotalTheory ssrbool.
+Open Scope order_scope.
+
+Context `{!heapGS Σ}.
+Context {d : Order.disp_t} {A : orderType d} `{!Repr A, !EqDecision A}.
+Context (i : A -> A) (eqv invv lev : val).
+
+Hypothesis eqvP : forall (x y : A) E Ψ,
+  Ψ #(bool_decide (x = y)) ⊢ WP eqv (repr x) (repr y) @ E [{ Ψ }].
+Hypothesis invvP : forall (x : A) E Ψ,
+  Ψ (repr (i x)) ⊢ WP invv (repr x) @ E [{ Ψ }].
+
+(* Stdpp packaging of the mathcomp order [<=%O] (cf. [pt_order] in
+   [core/pre_term/with_stdpp.v]). *)
+Definition ole : relation A := fun x y => is_true (x <= y).
+
+Global Instance ole_dec : RelDecision ole.
+Proof. rewrite /ole /RelDecision => x y; case: (x <= y); [by left | by right]. Qed.
+Global Instance ole_refl : Reflexive ole.
+Proof. move=> x; exact: lexx. Qed.
+Global Instance ole_trans : Transitive ole.
+Proof. move=> x y z; exact: le_trans. Qed.
+Global Instance ole_total : Total ole.
+Proof. by move=> x y; case/orP: (le_total x y); [left | right]. Qed.
+Global Instance ole_antisymm : AntiSymm eq ole.
+Proof. move=> x y Hxy Hyx; apply: le_anti; apply/andP; by split. Qed.
+
+Lemma sorted_StronglySorted_ole (l : list A) :
+  is_true (path.sorted <=%O l) -> StronglySorted ole l.
+Proof.
+elim: l => [_|x l IH]; first by constructor.
+move=> Hs.
+have Hl : is_true (path.sorted <=%O l) := path.path_sorted Hs.
+have Ha : is_true (seq.all (<=%O x) l) := path.order_path_min le_trans Hs.
+constructor; first exact: IH Hl.
+by elim: l Ha {IH Hl Hs} => [//|y l IH] /ssrbool.andP [xy /IH ?]; constructor.
+Qed.
+
+(* Bridge: mathcomp's [path.sort <=%O] and stdpp's [merge_sort ole] are both
+   *the* sorted permutation of the input, so they coincide. *)
+Lemma sort_merge_sort_ole (l : list A) :
+  path.sort <=%O l = merge_sort ole l.
+Proof.
+have Hss : StronglySorted ole (path.sort <=%O l).
+  apply: sorted_StronglySorted_ole; exact: (path.sort_sorted le_total).
+rewrite -{1}(merge_sort_id _ _ Hss).
+apply: merge_sort_Permutation_eq.
+apply/perm_Perm; rewrite path.perm_sort; exact: seq.perm_refl.
+Qed.
+
+(* The order-comparison closure still speaks mathcomp's [<=%O] (bool); this is
+   the last mathcomp-flavoured bit of the interface, to be replaced by a stdpp
+   [bool_decide (ole _ _)] once [twp_insertion_sort] is restated. *)
+Hypothesis levP : forall (x y : A) E Ψ,
+  Ψ #((x <= y)%O) ⊢ WP lev (repr x) (repr y) @ E [{ Ψ }].
+
+(* Correctness of [insertion_sort], restated in stdpp terms. *)
+Lemma twp_insertion_sort_merge (l : list A) E Ψ :
+  Ψ (repr (merge_sort ole l)) ⊢ WP insertion_sort lev (repr l) @ E [{ Ψ }].
+Proof.
+iIntros "HΨ".
+wp_apply (twp_insertion_sort d A lev l) => //.
+{ by iIntros "%x %y %Φ _ HΦ"; wp_apply levP; iApply "HΦ". }
+iIntros "_"; rewrite sort_merge_sort_ole; by iApply "HΨ".
+Qed.
+
+Lemma twp_sms_to xs E Ψ :
+  Ψ (repr (SMS.to ole i xs)) ⊢ WP sms_to lev eqv invv (repr xs) @ E [{ Ψ }].
+Proof.
+iIntros "HΨ"; wp_lam; wp_pures.
+wp_apply (twp_sms_cancel (i := i)); try exact: eqvP; try exact: invvP.
+wp_apply twp_insertion_sort_merge.
+rewrite /SMS.to; by iApply "HΨ".
+Qed.
+
+End Ordered.
